

## Quadriken

Für jedes  $t \in \mathbb{R}$  sei die Quadrik  $Q_t$  definiert durch:

$$Q_t: \left\{ \begin{pmatrix} x_1 \\ x_2 \end{pmatrix} \in \mathbb{R}^2 \mid 4x_1^2 + 4x_2^2 - 4x_1x_2 - 12x_1 + t = 0 \right\}$$

$$x^T A x + 2a^T x + c = 0$$

$$4x_1^2 + 4x_2^2 - 4x_1x_2 \Rightarrow A = \begin{pmatrix} 4 & -2 \\ -2 & 4 \end{pmatrix}$$

$$-12x_1 \Rightarrow \begin{pmatrix} -6 \\ 0 \end{pmatrix} = a$$

$$c = t$$

$$\chi_A(\lambda) = \det(A - \lambda E_2) = \begin{vmatrix} 4-\lambda & -2 \\ -2 & 4-\lambda \end{vmatrix} = (4-\lambda)^2 - 4$$

$$\chi_A(\lambda) \stackrel{!}{=} 0 \Rightarrow (4-\lambda)^2 = 2^2 \Rightarrow 4-\lambda = \pm 2$$

$$\Rightarrow \begin{cases} \lambda_2 = 4 + 2 = 6 \\ \lambda_1 = 4 - 2 = 2 \end{cases}$$

$$\lambda_2 = 6 \Rightarrow (A - 6E_2) \cdot x = 0 \Rightarrow \left[ \begin{array}{cc|c} 4-6 & -2 & 0 \\ -2 & 4-6 & 0 \end{array} \right] \Rightarrow$$

$$\Rightarrow \left[ \begin{array}{cc|c} -2 & -2 & 0 \\ -2 & -2 & 0 \end{array} \right] \Rightarrow \left[ \begin{array}{cc|c} -1 & -1 & 0 \\ 0 & 0 & 0 \end{array} \right] \Rightarrow \left[ \begin{array}{cc|c} 1 & 1 & 0 \\ 0 & 0 & 0 \end{array} \right]$$

$$Z_1: x_1 + x_2 = 0 \Rightarrow x_1 = -x_2 \Rightarrow v_2 = \begin{pmatrix} 1 \\ -1 \end{pmatrix}$$

$$\lambda_1 = 2 \Rightarrow (A - 2E_2) \cdot x = 0 \Rightarrow \left[ \begin{array}{cc|c} 4-2 & -2 & 0 \\ -2 & 4-2 & 0 \end{array} \right] \Rightarrow$$

$$\Rightarrow \left[ \begin{array}{cc|c} 2 & -2 & 0 \\ -2 & 2 & 0 \end{array} \right] \Rightarrow \left[ \begin{array}{cc|c} 2 & -2 & 0 \\ 4 & -2 & 0 \end{array} \right] \Rightarrow \left[ \begin{array}{cc|c} 1 & -1 & 0 \\ 0 & 0 & 0 \end{array} \right]$$



$$Z_1: x_1 - x_2 = 0 \Rightarrow x_1 = x_2 \Rightarrow v_1 = \begin{pmatrix} 1 \\ 1 \end{pmatrix}$$

$$\hat{v}_1 = \frac{v_1}{|v_1|} = \frac{1}{\sqrt{1^2+1^2}} \begin{pmatrix} 1 \\ 1 \end{pmatrix} = \frac{1}{\sqrt{2}} \begin{pmatrix} 1 \\ 1 \end{pmatrix}$$

$$\hat{v}_2 = \frac{v_2}{|v_2|} = \frac{1}{\sqrt{1^2+1^2}} \begin{pmatrix} 1 \\ -1 \end{pmatrix} = \frac{1}{\sqrt{2}} \begin{pmatrix} 1 \\ -1 \end{pmatrix}$$

$$F = (0, \hat{v}_1, \hat{v}_2)$$

$$\Leftrightarrow F = \left( 0, \frac{1}{\sqrt{2}} \begin{pmatrix} 1 \\ 1 \end{pmatrix}, \frac{1}{\sqrt{2}} \begin{pmatrix} 1 \\ -1 \end{pmatrix} \right)$$

$$\text{und } F = \frac{1}{\sqrt{2}} \begin{pmatrix} 1 & 1 \\ 1 & -1 \end{pmatrix} = E K_F$$

$$\Rightarrow 0 = y^T (F^T A F) y + z (F^T a)^T y + t$$

$$= (y_1, y_2) \left( \frac{1}{\sqrt{2}} \begin{pmatrix} 1 & 1 \\ 1 & -1 \end{pmatrix} \begin{pmatrix} 4 & -2 \\ -2 & 4 \end{pmatrix} \frac{1}{\sqrt{2}} \begin{pmatrix} 1 & 1 \\ 1 & -1 \end{pmatrix} \right) \begin{pmatrix} y_1 \\ y_2 \end{pmatrix} +$$

$$+ z \left( \frac{1}{\sqrt{2}} \begin{pmatrix} 1 & 1 \\ 1 & -1 \end{pmatrix} \begin{pmatrix} -6 \\ 0 \end{pmatrix} \right)^T (y_1, y_2) + t$$

$$= (y_1, y_2) \left( \frac{1}{2} \begin{pmatrix} 1 & 1 \\ 1 & -1 \end{pmatrix} \begin{pmatrix} 2 & 6 \\ 2 & -6 \end{pmatrix} \begin{pmatrix} 1 & 1 \\ 1 & -1 \end{pmatrix} \right) \begin{pmatrix} y_1 \\ y_2 \end{pmatrix} + z \cdot \frac{1}{\sqrt{2}} \begin{pmatrix} -6 \\ -6 \end{pmatrix}^T$$

$$\cdot (y_1, y_2) + t$$

$$= (y_1, y_2) \left( \frac{1}{2} \begin{pmatrix} 4 & 0 \\ 0 & 4 \end{pmatrix} \right) \begin{pmatrix} y_1 \\ y_2 \end{pmatrix} + \frac{1}{\sqrt{2}} (-12, -12) y + t$$

$$= (y_1, y_2) \begin{pmatrix} 2 & 0 \\ 0 & 2 \end{pmatrix} \begin{pmatrix} y_1 \\ y_2 \end{pmatrix} + (-6\sqrt{2}, -6\sqrt{2}) \begin{pmatrix} y_1 \\ y_2 \end{pmatrix} + t$$

$$= 2y_1^2 + 2y_2^2 - 6\sqrt{2}y_1 - 6\sqrt{2}y_2 + t$$



$$0 = 2y_1^2 - 6\sqrt{2}y_1 - 6y_2^2 - 6\sqrt{2}y_2 + t$$

$$= 2\left(y_1 - \frac{3\sqrt{2}}{2}\right)^2 - 9 + (6y_2 - 3\sqrt{2})^2 - 3 + t$$

$$= 2\left(y_1 - \frac{3\sqrt{2}}{2}\right)^2 + 6\left(y_2 - \frac{\sqrt{2}}{2}\right)^2 + t - 12$$

~~Sei~~

$$\text{Sei } z_1 = y_1 - \frac{3\sqrt{2}}{2}$$

$$z_2 = y_2 - \frac{\sqrt{2}}{2}$$

$$\Rightarrow 2z_1^2 + 6z_2^2 + t - 12 = 0$$

Fall 1:  $t = 12$

$$\Rightarrow \text{Euklidische Normalform: } 2z_1^2 + 6z_2^2 = 0$$

Fall 2:  $t \neq 12, t < 12$

$$\Rightarrow 2z_1^2 + 6z_2^2 + (t - 12) = 0 \quad | \cdot \frac{1}{t-12}$$

$$\Rightarrow \frac{2}{t-12} \cdot z_1^2 + \frac{6}{t-12} \cdot z_2^2 + 1 = 0$$